Split up unification, progressed towards proof

01Unification/Unification.thy
@@ -1,191 +1,171 @@
 theory Unification
-  imports "../00Utils/Utils"
+  imports Substitution
 begin
 
-datatype expr = 
-  Var string
-  | Ctor string "expr list"
-
-type_synonym subst = "string \<rightharpoonup> expr"
-
-primrec subst :: "subst \<Rightarrow> expr \<Rightarrow> expr" where
-  "subst s (Var x) = (case s x of Some e \<Rightarrow> e | None \<Rightarrow> Var x)"
-| "subst s (Ctor k es) = Ctor k (map (subst s) es)"
-
-definition extend_subst :: "string \<Rightarrow> expr \<Rightarrow> subst \<Rightarrow> subst" where
-  "extend_subst x e s y = (if x = y then Some e else map_option (subst [x \<mapsto> e]) (s y))"
-
-definition extension :: "subst \<Rightarrow> subst \<Rightarrow> bool" (infix "extends" 50) where
-  "s' extends s = (\<exists>xes. s' = fold (\<lambda>(x, e). extend_subst x e) xes s)"
-
-fun vars :: "expr \<Rightarrow> string set" 
-and varss :: "expr list \<Rightarrow> string set" where
-  "vars (Var x) = {x}"
-| "vars (Ctor k es) = varss es"
-| "varss [] = {}"
-| "varss (e # es) = vars e \<union> varss es"
-
-primrec ctors :: "expr \<Rightarrow> nat" where
-  "ctors (Var x) = 0"
-| "ctors (Ctor k es) = Suc (list_sum (map ctors es))"
-
-fun list_subst :: "string \<Rightarrow> expr \<Rightarrow> (expr \<times> expr) list \<Rightarrow> (expr \<times> expr) list" where
-  "list_subst x e' [] = []"
-| "list_subst x e' ((e\<^sub>1, e\<^sub>2) # ess) = (subst [x \<mapsto> e'] e\<^sub>1, subst [x \<mapsto> e'] e\<^sub>2) # list_subst x e' ess"
-
-fun list_vars :: "(expr \<times> expr) list \<Rightarrow> string set" where
-  "list_vars [] = {}"
-| "list_vars ((e\<^sub>1, e\<^sub>2) # ess) = vars e\<^sub>1 \<union> vars e\<^sub>2 \<union> list_vars ess"
-
-fun list_ctors :: "(expr \<times> expr) list \<Rightarrow> nat" where
-  "list_ctors [] = 0"
-| "list_ctors ((e\<^sub>1, e\<^sub>2) # ess) = ctors e\<^sub>1 + ctors e\<^sub>2 + list_ctors ess"
-
-abbreviation unifier :: "subst \<Rightarrow> expr \<Rightarrow> expr \<Rightarrow> bool" (infix "unifies _ and" 50) where 
-  "unifier s e\<^sub>1 e\<^sub>2 \<equiv> subst s e\<^sub>1 = subst s e\<^sub>2"
-
-fun list_unifier :: "subst \<Rightarrow> (expr \<times> expr) list \<Rightarrow> bool" (infix "unifies\<^sub>l" 50) where 
-  "list_unifier s [] = True"
-| "list_unifier s ((e\<^sub>1, e\<^sub>2) # ess) = ((s unifies e\<^sub>1 and e\<^sub>2) \<and> list_unifier s ess)"
+fun unify_induct :: "(expr \<times> expr) list \<Rightarrow> bool" where
+  "unify_induct [] = True"
+| "unify_induct ((Ctor k\<^sub>1 es\<^sub>1, Ctor k\<^sub>2 es\<^sub>2) # ess) = unify_induct ess"
+| "unify_induct ((Ctor k es, Var x) # ess) = unify_induct ess"
+| "unify_induct ((Var x, Ctor k es) # ess) = unify_induct ess"
+| "unify_induct ((Var x, Var y) # ess) = unify_induct ess"
 
 function unify' :: "(expr \<times> expr) list \<Rightarrow> subst \<rightharpoonup> subst" where
   "unify' [] s = Some s"
-| "unify' ((Ctor k\<^sub>1 es\<^sub>1, Ctor k\<^sub>2 es\<^sub>2) # ess) s = (
-    if k\<^sub>1 = k\<^sub>2 \<and> length es\<^sub>1 = length es\<^sub>2 then unify' (zip es\<^sub>1 es\<^sub>2 @ ess) s 
-    else None)"
-| "unify' ((Ctor k es, Var x) # ess) s = (
-    if x \<in> varss es then None
-    else unify' (list_subst x (Ctor k es) ess) (extend_subst x (Ctor k es) s))"
-| "unify' ((Var x, Ctor k es) # ess) s = (
-    if x \<in> varss es then None
-    else unify' (list_subst x (Ctor k es) ess) (extend_subst x (Ctor k es) s))"
-| "unify' ((Var x, Var y) # ess) s = unify' (list_subst x (Var y) ess) (extend_subst x (Var y) s)"
-  by pat_completeness auto
+| "k\<^sub>1 = k\<^sub>2 \<Longrightarrow> length es\<^sub>1 = length es\<^sub>2 \<Longrightarrow> unify' ((Ctor k\<^sub>1 es\<^sub>1, Ctor k\<^sub>2 es\<^sub>2) # ess) s = 
+    unify' (zip es\<^sub>1 es\<^sub>2 @ ess) s"
+| "k\<^sub>1 \<noteq> k\<^sub>2 \<or> length es\<^sub>1 \<noteq> length es\<^sub>2 \<Longrightarrow> unify' ((Ctor k\<^sub>1 es\<^sub>1, Ctor k\<^sub>2 es\<^sub>2) # ess) s = None"
+| "x \<in> varss es \<Longrightarrow> unify' ((Ctor k es, Var x) # ess) s = None"
+| "x \<notin> varss es \<Longrightarrow> unify' ((Ctor k es, Var x) # ess) s = 
+    unify' (list_subst x (Ctor k es) ess) (extend_subst x (Ctor k es) s)"
+| "x \<in> varss es \<Longrightarrow> unify' ((Var x, Ctor k es) # ess) s = None"
+| "x \<notin> varss es \<Longrightarrow> unify' ((Var x, Ctor k es) # ess) s = 
+    unify' (list_subst x (Ctor k es) ess) (extend_subst x (Ctor k es) s)"
+| "x = y \<Longrightarrow> unify' ((Var x, Var y) # ess) s = unify' ess s"
+| "x \<noteq> y \<Longrightarrow> unify' ((Var x, Var y) # ess) s = 
+    unify' (list_subst x (Var y) ess) (extend_subst x (Var y) s)"
+proof -
+  fix P 
+  fix x :: "(expr \<times> expr) list \<times> subst"
+  assume A: "(\<And>s. x = ([], s) \<Longrightarrow> P)" and 
+    B: "(\<And>k\<^sub>1 k\<^sub>2 es\<^sub>1 es\<^sub>2 ess s. k\<^sub>1 = k\<^sub>2 \<Longrightarrow> length es\<^sub>1 = length es\<^sub>2 \<Longrightarrow> 
+      x = ((Ctor k\<^sub>1 es\<^sub>1, Ctor k\<^sub>2 es\<^sub>2) # ess, s) \<Longrightarrow> P)" and 
+    C: "(\<And>k\<^sub>1 k\<^sub>2 es\<^sub>1 es\<^sub>2 ess s. k\<^sub>1 \<noteq> k\<^sub>2 \<or> length es\<^sub>1 \<noteq> length es\<^sub>2 \<Longrightarrow> 
+      x = ((Ctor k\<^sub>1 es\<^sub>1, Ctor k\<^sub>2 es\<^sub>2) # ess, s) \<Longrightarrow> P)" and
+    D: "(\<And>xa es k ess s. xa \<in> varss es \<Longrightarrow> x = ((Ctor k es, Var xa) # ess, s) \<Longrightarrow> P)" and
+    E: "(\<And>xa es k ess s. xa \<notin> varss es \<Longrightarrow> x = ((Ctor k es, Var xa) # ess, s) \<Longrightarrow> P)" and
+    F: "(\<And>xa es k ess s. xa \<in> varss es \<Longrightarrow> x = ((Var xa, Ctor k es) # ess, s) \<Longrightarrow> P)" and
+    G: "(\<And>xa es k ess s. xa \<notin> varss es \<Longrightarrow> x = ((Var xa, Ctor k es) # ess, s) \<Longrightarrow> P)" and
+    H: "(\<And>xa y ess s. xa = y \<Longrightarrow> x = ((Var xa, Var y) # ess, s) \<Longrightarrow> P)" and
+    I: "(\<And>xa y ess s. xa \<noteq> y \<Longrightarrow> x = ((Var xa, Var y) # ess, s) \<Longrightarrow> P)"
+  show P
+  proof (cases x)
+    case (Pair ess s)
+    with A B C D E F G H I show ?thesis 
+    proof (induction ess rule: unify_induct.induct)
+      case (2 k\<^sub>1 es\<^sub>1 k\<^sub>2 es\<^sub>2 ess)
+      thus ?case by (cases "k\<^sub>1 = k\<^sub>2 \<and> length es\<^sub>1 = length es\<^sub>2") auto
+    next
+      case (3 k es x ess)
+      thus ?case by (cases "x \<in> varss es") simp_all
+    next
+      case (4 x k es ess)
+      thus ?case by (cases "x \<in> varss es") simp_all
+    next
+      case (5 x y ess)
+      thus ?case by (cases "x = y") simp_all
+    qed simp_all
+  qed
+qed auto
+termination
+  by (relation "measures [card \<circ> list_vars \<circ> fst, list_ctor_count \<circ> fst, length \<circ> fst]") 
+     (simp_all add: card_insert_if)
 
 definition unify :: "expr \<Rightarrow> expr \<rightharpoonup> subst" where
   "unify e\<^sub>1 e\<^sub>2 = unify' [(e\<^sub>1, e\<^sub>2)] Map.empty"
 
-lemma [simp]: "finite (vars e)"
-  and [simp]: "finite (varss es)"
-  by (induction e and es rule: vars_varss.induct) simp_all
-
-lemma [simp]: "finite (list_vars ess)"
-  by (induction ess rule: list_vars.induct) simp_all
-
-lemma [simp]: "list_vars (ess\<^sub>1 @ ess\<^sub>2) = list_vars ess\<^sub>1 \<union> list_vars ess\<^sub>2"
-  by (induction ess\<^sub>1 rule: list_ctors.induct) auto
-
-lemma [simp]: "length es\<^sub>1 = length es\<^sub>2 \<Longrightarrow> list_vars (zip es\<^sub>1 es\<^sub>2) = varss es\<^sub>1 \<union> varss es\<^sub>2"
-proof (induction es\<^sub>1 arbitrary: es\<^sub>2)
-  case (Cons e\<^sub>1 es\<^sub>1)
-  thus ?case by (induction es\<^sub>2) auto
-qed simp_all
-
-lemma [simp]: "list_ctors (ess\<^sub>1 @ ess\<^sub>2) = list_ctors ess\<^sub>1 + list_ctors ess\<^sub>2"
-  by (induction ess\<^sub>1 rule: list_ctors.induct) simp_all
-
-lemma [simp]: "length es\<^sub>1 = length es\<^sub>2 \<Longrightarrow> 
-  list_ctors (zip es\<^sub>1 es\<^sub>2) = list_sum (map ctors es\<^sub>1) + list_sum (map ctors es\<^sub>2)"
-proof (induction es\<^sub>1 arbitrary: es\<^sub>2)
-  case (Cons e\<^sub>1 es\<^sub>1)
-  thus ?case by (induction es\<^sub>2) simp_all
-qed simp_all
-
-lemma [simp]: "subst [x \<mapsto> Var x] e = e"
-proof (induction e)
-  case (Ctor k es)
-  thus ?case by (induction es) simp_all
-qed simp_all
-
-lemma [simp]: "list_subst x (Var x) ess = ess"
-  by (induction x "Var x" ess rule: list_subst.induct) simp_all
-
-lemma [simp]: "x \<notin> vars e \<Longrightarrow> vars (subst [x \<mapsto> e'] e) = vars e"
-  and [simp]: "x \<notin> varss es \<Longrightarrow> varss (map (subst [x \<mapsto> e']) es) = varss es"
-  by (induction e and es rule: vars_varss.induct) simp_all
-
-lemma [simp]: "x \<in> vars e \<Longrightarrow> vars (subst [x \<mapsto> e'] e) = vars e - {x} \<union> vars e'"
-  and [simp]: "x \<in> varss es \<Longrightarrow> varss (map (subst [x \<mapsto> e']) es) = varss es - {x} \<union> vars e'"
-proof (induction e and es rule: vars_varss.induct)
-  case (4 e es)
-  hence "varss (map (subst [x \<mapsto> e']) (e # es)) = varss (e # es) - {x} \<union> vars e'" 
-    by fastforce
-  thus ?case by blast
-qed simp_all
-
-lemma [simp]: "vars (subst [x \<mapsto> e'] e) = vars e - {x} \<union> (if x \<in> vars e then vars e' else {})"
-  by simp
-
-lemma [simp]: "x \<notin> list_vars ess \<Longrightarrow> list_vars (list_subst x e ess) = list_vars ess"
-  by (induction ess rule: list_vars.induct) simp_all
-
-lemma [simp]: "x \<in> list_vars ess \<Longrightarrow> list_vars (list_subst x e ess) = list_vars ess - {x} \<union> vars e"
-proof (induction ess rule: list_vars.induct)
-  case (2 e\<^sub>1 e\<^sub>2 ess)
-  thus ?case by (cases "x \<in> list_vars ess") auto
-qed simp_all
-
-lemma [simp]: "list_vars (list_subst x e ess) = 
-    list_vars ess - {x} \<union> (if x \<in> list_vars ess then vars e else {})"
-  by simp
-
-lemma [simp]: "length (list_subst x e ess) = length ess"
-  by (induction x e ess rule: list_subst.induct) simp_all
-
-lemma [simp]: "ctors (subst [x \<mapsto> Var y] e) = ctors e"
-proof (induction e)
-  case (Ctor k es)
-  thus ?case by (induction es) simp_all
-qed simp_all
-
-lemma [simp]: "list_ctors (list_subst x (Var y) ess) = list_ctors ess"
-  by (induction x "Var y" ess rule: list_subst.induct) simp_all
-
-termination unify'
-  by (relation "measures [card \<circ> list_vars \<circ> fst, list_ctors \<circ> fst, length \<circ> fst]") 
-     (simp_all add: card_insert_if)
-
-lemma [simp]: "s unifies\<^sub>l (as @ bs) = ((s unifies\<^sub>l as) \<and> (s unifies\<^sub>l bs))"
-  by (induction s as rule: list_unifier.induct) simp_all
-
-lemma [simp]: "length es\<^sub>1 = length es\<^sub>2 \<Longrightarrow> 
-    (s unifies\<^sub>l zip es\<^sub>1 es\<^sub>2) = (map (subst s) es\<^sub>1 = map (subst s) es\<^sub>2)"
-proof (induction es\<^sub>1 arbitrary: es\<^sub>2)
-  case (Cons e es\<^sub>1)
-  thus ?case by (induction es\<^sub>2) simp_all
-qed simp_all
-
-lemma unify_none [simp]: "unify' ess s = None \<Longrightarrow> \<nexists>s'. s' extends s \<and> s' unifies\<^sub>l ess"
+lemma unify_ordered [simp]: "ordered_subst s \<Longrightarrow> dom s \<inter> list_vars ess = {} \<Longrightarrow> 
+    unify' ess s = Some s' \<Longrightarrow> ordered_subst s'"
 proof (induction ess s rule: unify'.induct)
-  case (2 k\<^sub>1 es\<^sub>1 k\<^sub>2 es\<^sub>2 ess s)
-  thus ?case by (cases "k\<^sub>1 = k\<^sub>2 \<and> length es\<^sub>1 = length es\<^sub>2") simp_all
+  case (5 x es k ess s)
+  moreover hence "vars (Ctor k es) \<inter> dom s = {}" by auto
+  moreover from 5 have "dom (extend_subst x (Ctor k es) s) \<inter> 
+    list_vars (list_subst x (Ctor k es) ess) = {}" by auto
+  ultimately show ?case by simp
 next
-  case (3 k es x ess s)
-  thus ?case by simp
+  case (7 x es k ess s)
+  moreover hence "vars (Ctor k es) \<inter> dom s = {}" by auto
+  moreover from 7 have "dom (extend_subst x (Ctor k es) s) \<inter> 
+    list_vars (list_subst x (Ctor k es) ess) = {}" by auto
+  ultimately show ?case by simp
 next
-  case (4 x k es ess s)
-  thus ?case by simp
-next
-  case (5 x y ess s)
-  from 5 have "\<nexists>s'. s' unifies\<^sub>l list_subst x (Var y) ess" by simp
-  from 5 have "unify' (list_subst x (Var y) ess) (extend_subst x (Var y) s) = None" by simp
-
-
-  have "\<forall>s'. (case s' x of None \<Rightarrow> Var x | Some e \<Rightarrow> e) = (case s' y of None \<Rightarrow> Var y | Some e \<Rightarrow> e) \<longrightarrow> \<not> s' unifies\<^sub>l ess" by simp
-  thus ?case by simp
+  case (9 x y ess s)
+  moreover hence "dom (extend_subst x (Var y) s) \<inter> list_vars (list_subst x (Var y) ess) = {}"
+    by auto
+  ultimately show ?case by simp
 qed simp_all
 
-lemma [simp]: "s extends Map.empty"
-  by (unfold extension_def)
+lemma [simp]: "unify e\<^sub>1 e\<^sub>2 = Some s \<Longrightarrow> ordered_subst s"
+proof (unfold unify_def)
+  assume "unify' [(e\<^sub>1, e\<^sub>2)] Map.empty = Some s"
+  moreover have "ordered_subst Map.empty" by simp
+  moreover have "dom Map.empty \<inter> list_vars [(e\<^sub>1, e\<^sub>2)] = {}" by simp
+  ultimately show "ordered_subst s" by (metis unify_ordered)
+qed
+
+lemma unify_none [simp]: "unify' ess s = None \<Longrightarrow> \<nexists>s'. s' unifies\<^sub>l ess"
+proof (induction ess s rule: unify'.induct)
+  case (2 k\<^sub>1 k\<^sub>2 es\<^sub>1 es\<^sub>2 ess s)
+  then show ?case by simp
+next
+  case (4 x es k ess s)
+  then show ?case by simp
+next
+  case (5 x es k ess s)
+  then show ?case by simp
+next
+  case (6 x es k ess s)
+  then show ?case by simp
+next
+  case (7 x es k ess s)
+  then show ?case by simp
+next
+  case (9 x y ess s)
+  from 9 have "x \<noteq> y" by simp
+  from 9 have "\<And>s'. \<not> s' unifies\<^sub>l list_subst x (Var y) ess" by simp
+  from 9 have "unify' (list_subst x (Var y) ess) (extend_subst x (Var y) s) = None" by simp
+
+
+  have "\<And>s'. (\<not> s' unifies Var x and Var y) \<or> \<not> s' unifies\<^sub>l ess" by simp
+  then show ?case by simp
+qed simp_all
 
 lemma [simp]: "unify e\<^sub>1 e\<^sub>2 = None \<Longrightarrow> \<nexists>s. s unifies e\<^sub>1 and e\<^sub>2"
 proof (unfold unify_def)
   assume "unify' [(e\<^sub>1, e\<^sub>2)] Map.empty = None"
-  hence "\<nexists>s'. s' extends Map.empty \<and> s' unifies\<^sub>l [(e\<^sub>1, e\<^sub>2)]" by (metis unify_none)
+  hence "\<nexists>s'. s' unifies\<^sub>l [(e\<^sub>1, e\<^sub>2)]" by (metis unify_none)
   thus "\<nexists>s. s unifies e\<^sub>1 and e\<^sub>2" by simp
 qed
 
-lemma [simp]: "unify e\<^sub>1 e\<^sub>2 = Some s \<Longrightarrow> (s unifies e\<^sub>1 and e\<^sub>2)"
-  by simp
+lemma unify_some [simp]: "ordered_subst s \<Longrightarrow> sdom s \<inter> list_vars ess = {} \<Longrightarrow> 
+  unify' ess s = Some s' \<Longrightarrow> s' unifies\<^sub>l ess"
+proof (induction ess s rule: unify'.induct)
+  case (2 k\<^sub>1 k\<^sub>2 es\<^sub>1 es\<^sub>2 ess s)
+  then show ?case by simp
+next
+  case (5 x es k ess s)
+  then show ?case by simp
+next
+  case (7 x es k ess s)
+  then show ?case by simp
+next
+  case (9 x y ess s)
+  hence "unify' (list_subst x (Var y) ess) ((x, Var y) # s) = Some s'" by simp
+  then obtain s'' where S: "s' = s'' @ (x, Var y) # s" by fastforce
+
+  with 9 have O: "ordered_subst s'" by (metis unify_ordered)
+
+  from 9 have "sdom s \<inter> list_vars (list_subst x (Var y) ess) = {}" by auto
+  with 9 have "s' unifies\<^sub>l list_subst x (Var y) ess" by simp
+
+
+  from 9 have "x \<noteq> y" by simp
+  from 9 have "ordered_subst s" by simp
+  from 9 have "x \<notin> sdom s" by simp
+  from 9 have "y \<notin> sdom s" by simp
+  from 9 have "sdom s \<inter> list_vars ess = {}" by simp
+
+
+  have "s' unifies\<^sub>l ess" by simp
+  with S O show ?case by simp
+qed simp_all
+
+lemma [simp]: "unify e\<^sub>1 e\<^sub>2 = Some s \<Longrightarrow> s unifies e\<^sub>1 and e\<^sub>2"
+proof (unfold unify_def)
+  assume "unify' [(e\<^sub>1, e\<^sub>2)] Map.empty = Some s"
+  moreover have "ordered_subst Map.empty" by simp
+  moreover have "dom Map.empty \<inter> list_vars [(e\<^sub>1, e\<^sub>2)] = {}" by simp
+  ultimately have "s unifies\<^sub>l [(e\<^sub>1, e\<^sub>2)]" by (metis unify_some)
+  thus "s unifies e\<^sub>1 and e\<^sub>2" by simp
+qed
 
 end
