01Unification/Substitution.thy
@@ -1,0 +1,69 @@
+theory Substitution
+  imports UnifyExpr
+begin
+
+type_synonym subst = "string \<rightharpoonup> expr"
+
+fun subst :: "subst \<Rightarrow> expr \<Rightarrow> expr" where
+  "subst s (Var y) = (case s y of Some e \<Rightarrow> e | None \<Rightarrow> Var y)"
+| "subst s (Ctor k es) = Ctor k (map (subst s) es)"
+
+fun list_subst :: "string \<Rightarrow> expr \<Rightarrow> (expr \<times> expr) list \<Rightarrow> (expr \<times> expr) list" where
+  "list_subst x e' [] = []"
+| "list_subst x e' ((e\<^sub>1, e\<^sub>2) # ess) = (subst [x \<mapsto> e'] e\<^sub>1, subst [x \<mapsto> e'] e\<^sub>2) # list_subst x e' ess"
+
+abbreviation unifier :: "subst \<Rightarrow> expr \<Rightarrow> expr \<Rightarrow> bool" (infix "unifies _ and" 50) where 
+  "unifier s e\<^sub>1 e\<^sub>2 \<equiv> subst s e\<^sub>1 = subst s e\<^sub>2"
+
+fun list_unifier :: "subst \<Rightarrow> (expr \<times> expr) list \<Rightarrow> bool" (infix "unifies\<^sub>l" 50) where 
+  "list_unifier s [] = True"
+| "list_unifier s ((e\<^sub>1, e\<^sub>2) # ess) = ((s unifies e\<^sub>1 and e\<^sub>2) \<and> list_unifier s ess)"
+
+definition extend_subst :: "string \<Rightarrow> expr \<Rightarrow> subst \<Rightarrow> subst" where
+  "extend_subst x e s y = (if x = y then Some e else map_option (subst [x \<mapsto> e]) (s y))"
+
+definition ordered_subst :: "subst \<Rightarrow> bool" where
+  "ordered_subst s = (dom s \<inter> \<Union> (vars ` ran s) = {})"
+
+lemma [simp]: "x \<notin> vars e \<Longrightarrow> vars (subst [x \<mapsto> e'] e) = vars e"
+  and [simp]: "x \<notin> varss es \<Longrightarrow> varss (map (subst [x \<mapsto> e']) es) = varss es"
+  by (induction e and es rule: vars_varss.induct) simp_all
+
+lemma [simp]: "x \<in> vars e \<Longrightarrow> vars (subst [x \<mapsto> e'] e) = vars e - {x} \<union> vars e'"
+  and [simp]: "x \<in> varss es \<Longrightarrow> varss (map (subst [x \<mapsto> e']) es) = varss es - {x} \<union> vars e'"
+proof (induction e and es rule: vars_varss.induct)
+  case (4 e es)
+  hence "varss (map (subst [x \<mapsto> e']) (e # es)) = varss (e # es) - {x} \<union> vars e'" by fastforce
+  thus ?case by blast
+qed simp_all
+
+lemma [simp]: "vars (subst [x \<mapsto> e'] e) = vars e - {x} \<union> (if x \<in> vars e then vars e' else {})"
+  by simp
+
+lemma [simp]: "x \<notin> list_vars ess \<Longrightarrow> list_vars (list_subst x e ess) = list_vars ess"
+  by (induction ess rule: list_vars.induct) simp_all
+
+lemma [simp]: "x \<in> list_vars ess \<Longrightarrow> list_vars (list_subst x e ess) = list_vars ess - {x} \<union> vars e"
+proof (induction ess rule: list_vars.induct)
+  case (2 e\<^sub>1 e\<^sub>2 ess)
+  thus ?case by (cases "x \<in> list_vars ess") auto
+qed simp_all
+
+lemma [simp]: "list_vars (list_subst x e ess) = 
+    list_vars ess - {x} \<union> (if x \<in> list_vars ess then vars e else {})"
+  by simp
+
+lemma [simp]: "dom (extend_subst x e s) = insert x (dom s)"
+  by (auto simp add: extend_subst_def)
+
+lemma [simp]: "x \<notin> dom s \<Longrightarrow> ran (extend_subst x e s) = insert e (subst [x \<mapsto> e] ` ran s)"
+  by (auto simp add: extend_subst_def ran_def)
+
+lemma [simp]: "ordered_subst Map.empty"
+  by (simp add: ordered_subst_def)
+
+lemma [simp]: "ordered_subst s \<Longrightarrow> x \<notin> vars e \<Longrightarrow> vars e \<inter> dom s = {} \<Longrightarrow> x \<notin> dom s \<Longrightarrow> 
+    ordered_subst (extend_subst x e s)"
+  by (auto simp add: ordered_subst_def split: if_splits)
+
+end
