01Unification/UnifyExpr.thy
@@ -1,0 +1,54 @@
+theory UnifyExpr
+  imports "../00Utils/Utils"
+begin
+
+datatype expr = 
+  Var string
+  | Ctor string "expr list"
+
+fun vars :: "expr \<Rightarrow> string set" 
+and varss :: "expr list \<Rightarrow> string set" where
+  "vars (Var x) = {x}"
+| "vars (Ctor k es) = varss es"
+| "varss [] = {}"
+| "varss (e # es) = vars e \<union> varss es"
+
+primrec ctor_count :: "expr \<Rightarrow> nat" where
+  "ctor_count (Var x) = 0"
+| "ctor_count (Ctor k es) = Suc (list_sum (map ctor_count es))"
+
+fun list_vars :: "(expr \<times> expr) list \<Rightarrow> string set" where
+  "list_vars [] = {}"
+| "list_vars ((e\<^sub>1, e\<^sub>2) # ess) = vars e\<^sub>1 \<union> vars e\<^sub>2 \<union> list_vars ess"
+
+fun list_ctor_count :: "(expr \<times> expr) list \<Rightarrow> nat" where
+  "list_ctor_count [] = 0"
+| "list_ctor_count ((e\<^sub>1, e\<^sub>2) # ess) = ctor_count e\<^sub>1 + ctor_count e\<^sub>2 + list_ctor_count ess"
+
+lemma [simp]: "finite (vars e)"
+  and [simp]: "finite (varss es)"
+  by (induction e and es rule: vars_varss.induct) simp_all
+
+lemma [simp]: "finite (list_vars ess)"
+  by (induction ess rule: list_vars.induct) simp_all
+
+lemma [simp]: "list_vars (ess\<^sub>1 @ ess\<^sub>2) = list_vars ess\<^sub>1 \<union> list_vars ess\<^sub>2"
+  by (induction ess\<^sub>1 rule: list_ctor_count.induct) auto
+
+lemma [simp]: "length es\<^sub>1 = length es\<^sub>2 \<Longrightarrow> list_vars (zip es\<^sub>1 es\<^sub>2) = varss es\<^sub>1 \<union> varss es\<^sub>2"
+proof (induction es\<^sub>1 arbitrary: es\<^sub>2)
+  case (Cons e\<^sub>1 es\<^sub>1)
+  thus ?case by (induction es\<^sub>2) auto
+qed simp_all
+
+lemma [simp]: "list_ctor_count (ess\<^sub>1 @ ess\<^sub>2) = list_ctor_count ess\<^sub>1 + list_ctor_count ess\<^sub>2"
+  by (induction ess\<^sub>1 rule: list_ctor_count.induct) simp_all
+
+lemma [simp]: "length es\<^sub>1 = length es\<^sub>2 \<Longrightarrow> 
+  list_ctor_count (zip es\<^sub>1 es\<^sub>2) = list_sum (map ctor_count es\<^sub>1) + list_sum (map ctor_count es\<^sub>2)"
+proof (induction es\<^sub>1 arbitrary: es\<^sub>2)
+  case (Cons e\<^sub>1 es\<^sub>1)
+  thus ?case by (induction es\<^sub>2) simp_all
+qed simp_all
+
+end
